compiler/src/compiler/FlatToRiscvCommon.v
@@ -326,9 +326,18 @@ Section WithParameters.
          (finalL.(getMetrics) - initialL.(getMetrics) <=
           lowerMetrics (finalMetricsH - initialMetricsH))%metricsL /\
          goodMachine finalIOTrace finalMH finalRegsH g finalL /\
-           exists t' rt',
-             finalTrace = t' ++ initialTrace /\
-               getTrace finalL = rt' ++ getTrace initialL /\
+           exists k1'' k2'',
+             finalTrace = k1'' ++ initialTrace /\
+               getTrace finalL = k2'' ++ getTrace initialL /\
+               (forall k20 k1''' f,
+                   fst (rtransform_stmt_trace iset compile_ext_call leak_ext_call e_pos program_base e_impl_full
+                          (s, rev k1'' ++ k1''', k20, pos, g.(p_sp), (bytes_per_word * rem_framewords g), f)) =
+                     fst (f (rev k1'') (k20 ++ rev k2''))) /\
+               (forall k20 (*note how, unlike in 'spilling_correct_for', we don't use k20 for anything... it's just in the way.  strongly suggests I should get rid of it. *)k1''' f,
+                   predicts (fun k => snd (f (rev k1'' ++ k) (rev k1'') (k20 ++ rev k2''))) k1''' ->
+                   predicts (fun k => snd (rtransform_stmt_trace iset compile_ext_call leak_ext_call e_pos program_base e_impl_full
+                                             (s, k, k20, pos, g.(p_sp), (bytes_per_word * rem_framewords g), (f k)))) (rev k1'' ++ k1'''))).
+               
                forall a t'' f,
                  generates a (rev t' ++ t'') ->
                  rtransform_stmt_trace iset compile_ext_call leak_ext_call e_pos program_base e_impl_full
